MonadReturns overhaul. Splitting into more classes.

src/coq/Utils/MonadReturnsLaws.v
@@ -25,12 +25,6 @@ Section Laws.
 
       MFails : forall {A} (ma : M A), Prop;
 
-      MFails_MReturns : forall {A} (ma : M A),
-          MFails ma -> forall a, ~ MReturns a ma;
-
-      MReturns_MFails : forall {A} (ma : M A) (a : A),
-          MReturns a ma -> ~ MFails ma;
-
       MFails_ret : forall {A} (a : A),
           ~ MFails (ret a);
 
@@ -38,18 +32,57 @@ Section Laws.
           MReturns a ma -> MReturns b (k a) -> MReturns b (bind ma k);
 
       MReturns_bind_inv : forall {A B} (ma : M A) (k : A -> M B) (b : B),
-          MReturns b (bind ma k) -> exists a : A , MReturns a ma /\ MReturns b (k a);
+          MReturns b (bind ma k) -> (MFails ma \/ exists a : A , MReturns a ma /\ MReturns b (k a));
 
       MReturns_ret : forall {A} (a : A) (ma : M A),
-          ~MFails ma -> eq1 ma (ret a) -> MReturns a ma;
+          ~MFails ma -> eq1 (ret a) ma -> MReturns a ma;
 
       MReturns_ret_inv : forall {A} (x y : A),
           MReturns x (ret y) -> x = y;
+    }.
 
-      MReturns_Proper :> forall {A} (a : A),
-          Proper (eq1 ==> Basics.impl) (MReturns a)
-   }.
 End Laws.
+
+Arguments MReturns {M _ _ _ _}.
+Arguments MFails {M _ _ _ _}.
+Arguments MReturns_bind {M _ _ _ _}.
+Arguments MReturns_bind_inv {M _ _ _ _}.
+Arguments MReturns_ret {M _ _ _ _}.
+Arguments MReturns_ret_inv {M _ _ _ _}.
+
+Section ExtraLaws.
+  Context (M : Type -> Type).
+  Context {Monad : Monad M}.
+  Context {Eq1 : @Eq1 M}.
+  Context {MRET : @MonadReturns M Monad Eq1}.
+
+  (* Won't work when a refinement can fail and not return something *)
+  Class MonadReturnsProper :=
+    { MReturns_Proper :> forall {A} (a : A),
+          Proper (eq1 ==> Basics.impl) (MReturns a)
+    }.
+
+  (* These won't work with UB / Error refinement relations *)
+  Class MonadReturnsFails :=
+    {
+      MFails_MReturns : forall {A} (ma : M A),
+        MFails ma -> forall a, ~ MReturns a ma;
+
+      MReturns_MFails : forall {A} (ma : M A) (a : A),
+          MReturns a ma -> ~ MFails ma
+    }.
+
+  Class MonadReturnsStrongBindInv :=
+    {
+      MReturns_strong_bind_inv : forall {A B} (ma : M A) (k : A -> M B) (b : B),
+          MReturns b (bind ma k) -> exists a : A , MReturns a ma /\ MReturns b (k a);
+    }.
+
+End ExtraLaws.
+
+Arguments MFails_MReturns {M _ _ _ _}.
+Arguments MReturns_MFails {M _ _ _ _}.
+Arguments MReturns_strong_bind_inv {M _ _ _ _}.
 
 Section MReturns_ProperFlip.
   Context (M : Type -> Type).
@@ -59,9 +92,11 @@ Section MReturns_ProperFlip.
 
   Class MonadReturns_ProperFlip :=
     { MReturns_ProperFlip :> forall {A} (a : A),
-        Proper (eq1 ==> fun A B => Basics.impl B A) (MReturns _ a)
+        Proper (eq1 ==> fun A B => Basics.impl B A) (MReturns a)
     }.
 End MReturns_ProperFlip.
+
+Arguments MReturns_ProperFlip {M _ _ _ _}.
 
 Section MonadReturnsInv.
   Context (M : Type -> Type).
@@ -70,15 +105,10 @@ Section MonadReturnsInv.
   Context {MRET : @MonadReturns M Monad Eq1}.
   Class MonadReturns_Proper_inv :=
     { MReturns_Proper_inv :> forall {A} (a: A),
-        Proper ((fun (x y : M A) => MReturns M a x <-> MReturns M a y) ==> Monad.eq1) (fun x => x) }.
+        Proper ((fun (x y : M A) => MReturns a x <-> MReturns a y) ==> Monad.eq1) (fun x => x) }.
 End MonadReturnsInv.
 
-Arguments MReturns {M _ _ _ _}.
-Arguments MFails {M _ _ _ _}.
-Arguments MReturns_bind {M _ _ _ _}.
-Arguments MReturns_bind_inv {M _ _ _ _}.
-Arguments MReturns_ret {M _ _ _ _}.
-Arguments MReturns_ret_inv {M _ _ _ _}.
+Arguments MReturns_Proper_inv {M _ _ _ _}.
 
 Section NoFailsRet.
   Context (M : Type -> Type).
@@ -141,7 +171,7 @@ Section Sum.
     auto.
   Qed.
 
-  Lemma SumReturns_bind_inv :
+  Lemma SumReturns_strong_bind_inv :
     forall {A B} (ma : sum E A) (k : A -> sum E B) (b : B),
       SumReturns b (bind ma k) -> exists a : A , SumReturns a ma /\ SumReturns b (k a).
   Proof.
@@ -152,11 +182,23 @@ Section Sum.
       auto.
   Qed.
 
+  Lemma SumReturns_bind_inv :
+    forall {A B} (ma : sum E A) (k : A -> sum E B) (b : B),
+      SumReturns b (bind ma k) -> (SumFails ma \/ exists a : A , SumReturns a ma /\ SumReturns b (k a)).
+  Proof.
+    intros * Hb.
+    right. apply SumReturns_strong_bind_inv; auto.
+  Qed.
+
   Lemma SumReturns_ret :
     forall {A} (a : A) (ma : sum E A),
-      ~SumFails ma -> eq1 ma (ret a) -> SumReturns a ma.
+      ~SumFails ma -> eq1 (ret a) ma -> SumReturns a ma.
   Proof.
     intros * Hma.
+    intros H.
+    cbn in *.    
+    unfold SumReturns.
+    do 2 red in H.
     auto.
   Qed.
 
@@ -199,14 +241,20 @@ Section Sum.
   Global Instance MonadReturns_Sum : MonadReturns (sum E)
     := { MReturns := fun A => SumReturns;
          MFails := fun A => SumFails;
-         MReturns_MFails := fun A => SumReturns_SumFails;
-         MFails_MReturns := fun A => SumFails_SumReturns;
          MFails_ret := fun A => SumFails_ret;
          MReturns_bind := fun A B => SumReturns_bind;
          MReturns_bind_inv := fun A B => SumReturns_bind_inv;
          MReturns_ret := fun A => SumReturns_ret;
          MReturns_ret_inv := fun A => SumReturns_ret_inv
     }.
+
+  Global Instance MonadReturns_Sum_Fails : MonadReturnsFails (sum E)
+    := { MReturns_MFails := fun A => SumReturns_SumFails;
+         MFails_MReturns := fun A => SumFails_SumReturns
+    }.
+
+  Global Instance MonadReturns_Sum_StrongBindInv : MonadReturnsStrongBindInv (sum E)
+    := {  MReturns_strong_bind_inv := fun A B => SumReturns_strong_bind_inv }.
 
   Global Instance NoFailsRet_Sum : NoFailsRet (sum E).
   Proof.
@@ -271,7 +319,7 @@ Section Ident.
     reflexivity.
   Qed.
 
-  Lemma IdentReturns_bind_inv :
+  Lemma IdentReturns_strong_bind_inv :
     forall {A B} (ma : ident A) (k : A -> ident B) (b : B),
       IdentReturns b (bind ma k) -> exists a : A , IdentReturns a ma /\ IdentReturns b (k a).
   Proof.
@@ -281,9 +329,17 @@ Section Ident.
     exists a; split; auto.
   Qed.
 
+  Lemma IdentReturns_bind_inv :
+    forall {A B} (ma : ident A) (k : A -> ident B) (b : B),
+      IdentReturns b (bind ma k) -> (IdentFails ma \/ exists a : A , IdentReturns a ma /\ IdentReturns b (k a)).
+  Proof.
+    intros * Hb.
+    right; apply IdentReturns_strong_bind_inv; auto.
+  Qed.
+
   Lemma IdentReturns_ret :
     forall {A} (a : A) (ma : ident A),
-      ~IdentFails ma -> eq1 ma (ret a) -> IdentReturns a ma.
+      ~IdentFails ma -> eq1 (ret a) ma -> IdentReturns a ma.
   Proof.
     intros * NFAILS Hma.
     destruct ma as [a'].
@@ -326,14 +382,21 @@ Section Ident.
   Global Instance MonadReturns_Ident : MonadReturns ident
     := { MReturns := fun A => IdentReturns;
          MFails := fun A => IdentFails;
-         MReturns_MFails := fun A => IdentReturns_IdentFails;
-         MFails_MReturns := fun A => IdentFails_IdentReturns;
          MFails_ret := fun A => IdentFails_ret;
          MReturns_bind := fun A B => IdentReturns_bind;
          MReturns_bind_inv := fun A B => IdentReturns_bind_inv;
          MReturns_ret := fun A => IdentReturns_ret;
          MReturns_ret_inv := fun A => IdentReturns_ret_inv
        }.
+
+  Global Instance MonadReturns_Ident_Fails : MonadReturnsFails ident
+    := { MReturns_MFails := fun A => IdentReturns_IdentFails;
+         MFails_MReturns := fun A => IdentFails_IdentReturns
+    }.
+
+  Global Instance MonadReturns_Ident_StrongBindInv : MonadReturnsStrongBindInv ident
+    := {  MReturns_strong_bind_inv := fun A B => IdentReturns_strong_bind_inv }.
+
 
   Global Instance NoFailsRet_Ident : NoFailsRet (ident).
   Proof.
@@ -352,7 +415,9 @@ Section EitherT.
   Context {EQM : @Eq1 M}.
   Context {EQV : @Eq1Equivalence M HM EQM}.
   Context {MRET : @MonadReturns M HM EQM}.
-
+  Context {MRETF : @MonadReturnsFails M HM EQM MRET}.
+  Context {MRETP : @MonadReturnsProper M HM EQM MRET}.
+  Context {MRETSTR : @MonadReturnsStrongBindInv M HM EQM MRET}.
 
   Definition EitherTReturns {A} (a : A) (ma : eitherT E M A) : Prop
     := MReturns (inr a) (unEitherT ma).
@@ -368,7 +433,7 @@ Section EitherT.
     unfold EitherTFails in FAILS.
     intros CONTRA.
     unfold EitherTReturns in CONTRA.
-    eapply (MFails_MReturns M _ _ (inr a)); eauto.
+    eapply (MFails_MReturns _ _ _ (inr a) CONTRA); eauto.
     Unshelve.
     eauto.
   Qed.
@@ -399,22 +464,36 @@ Section EitherT.
     eapply MReturns_bind; eauto.
   Qed.
 
-  Lemma EitherTReturns_bind_inv :
+  Lemma EitherTReturns_strong_bind_inv :
     forall {A B} (ma : eitherT E M A) (k : A -> eitherT E M B) (b : B),
       EitherTReturns b (bind ma k) -> exists a : A , EitherTReturns a ma /\ EitherTReturns b (k a).
   Proof.
     intros * Hb.
     unfold EitherTReturns in *.
-    eapply MReturns_bind_inv in Hb as (ea & Ha & Hb).
+    eapply MReturns_strong_bind_inv in Hb as (ea & Ha & Hb).
     destruct ea; eauto.
 
     apply MReturns_ret_inv in Hb.
     inversion Hb.
   Qed.
 
+  Lemma EitherTReturns_bind_inv :
+    forall {A B} (ma : eitherT E M A) (k : A -> eitherT E M B) (b : B),
+      EitherTReturns b (bind ma k) -> (EitherTFails ma \/ exists a : A , EitherTReturns a ma /\ EitherTReturns b (k a)).
+  Proof.
+    intros * Hb.
+    unfold EitherTReturns in *.
+    eapply MReturns_bind_inv in Hb as [fails | (ea & Ha & Hb)].
+    + left; red; auto.
+    + destruct ea; eauto.
+
+      apply MReturns_ret_inv in Hb.
+      inversion Hb.
+  Qed.
+
   Lemma EitherTReturns_ret :
     forall {A} (a : A) (ma : eitherT E M A),
-      ~EitherTFails ma -> eq1 ma (ret a) -> EitherTReturns a ma.
+      ~EitherTFails ma -> eq1 (ret a) ma -> EitherTReturns a ma.
   Proof.
     intros * NFAILS Hma.
     eapply MReturns_ret; eauto.
@@ -459,14 +538,20 @@ Section EitherT.
   Global Instance MonadReturns_EitherT : MonadReturns (eitherT E M)
     := { MReturns := fun A => EitherTReturns;
          MFails := fun A => EitherTFails;
-         MReturns_MFails := fun A => EitherTReturns_EitherTFails;
-         MFails_MReturns := fun A => EitherTFails_EitherTReturns;
          MFails_ret := fun A => EitherTFails_ret;
          MReturns_bind := fun A B => EitherTReturns_bind;
          MReturns_bind_inv := fun A B => EitherTReturns_bind_inv;
          MReturns_ret := fun A => EitherTReturns_ret;
          MReturns_ret_inv := fun A => EitherTReturns_ret_inv
        }.
+
+  Global Instance MonadReturns_EitherT_Fails : MonadReturnsFails (eitherT E M)
+    := { MReturns_MFails := fun A => EitherTReturns_EitherTFails;
+         MFails_MReturns := fun A => EitherTFails_EitherTReturns
+    }.
+
+  Global Instance MonadReturns_EitherT_StrongBindInv : MonadReturnsStrongBindInv (eitherT E M)
+    := {  MReturns_strong_bind_inv := fun A B => EitherTReturns_strong_bind_inv }.
 
   Global Instance NoFailsRet_EitherT `{NFR : @NoFailsRet M HM EQM MRET} : NoFailsRet (eitherT E M).
   Proof.
@@ -511,7 +596,8 @@ Section StateT.
   Context {EQM : @Eq1 M}.
   Context {EQV : @Eq1Equivalence M HM EQM}.
   Context {MRET : @MonadReturns M HM EQM}.
-
+  Context {MRETF : @MonadReturnsFails M HM EQM MRET}.
+  Context {MRETSTR : @MonadReturnsStrongBindInv M HM EQM MRET}.
 
   Definition StateTReturns {A} (a : A) (ma : stateT S M A) : Prop
     := forall s, exists s', MReturns (a, s') (runStateT ma s).
@@ -541,7 +627,7 @@ Section StateT.
   (*   reflexivity. *)
   (* Qed. *)
 
-  Lemma StateTReturns_bind_inv :
+  Lemma StateTReturns_strong_bind_inv :
     forall {A B} (ma : stateT S M A) (k : A -> stateT S M B) (b : B),
       (forall s, exists sb, MReturns (b, sb) (runStateT (bind ma k) s)) -> forall s, exists (sa : S) (sb : S) (a : A), MReturns (a, sa) (runStateT ma s) /\ MReturns (b, sb) (runStateT (k a) sa).
   Proof.
@@ -549,8 +635,8 @@ Section StateT.
 
     specialize (H s) as (sb & RET).
     cbn in RET.
-    apply MReturns_bind_inv in RET as ((s' & b') & Hbind & Hb).
-    apply MReturns_bind_inv in Hbind as ((sa & a) & Hbind & Hb').
+    apply MReturns_strong_bind_inv in RET as ((s' & b') & Hbind & Hb).
+    apply MReturns_strong_bind_inv in Hbind as ((sa & a) & Hbind & Hb').
 
     exists sa. exists sb. exists a.
     split.
